coq_session/sta_uniq.v
@@ -48,10 +48,11 @@ Inductive head_sim : term -> term -> Prop :=
 | head_sim_send0 m : head_sim (Send0 m) (Send0 m)
 | head_sim_send1 m : head_sim (Send1 m) (Send1 m)
 | head_sim_close m : head_sim (Close m) (Close m)
-| head_sim_wait m : head_sim (Wait m) (Wait m).
+| head_sim_wait m : head_sim (Wait m) (Wait m)
+| head_sim_box : head_sim Box Box.
 
 Inductive sim (m n : term) : Prop :=
-| Sim x y : m === x -> head_sim x y -> y === n -> sim m n.
+| Sim x y : m ≃ x -> head_sim x y -> y ≃ n -> sim m n.
 
 Inductive sta_ctx_sim : sta_ctx -> sta_ctx -> Prop :=
 | sta_ctx_sim_nil : sta_ctx_sim nil nil
@@ -76,14 +77,14 @@ Lemma sim_reflexive m : sim m m.
 Proof with eauto. econstructor... Qed.
 #[global] Hint Resolve sim_reflexive.
 
-Lemma sim_transL x y z : sim x y -> y === z -> sim x z.
+Lemma sim_transL x y z : sim x y -> y ≃ z -> sim x z.
 Proof with eauto.
   move=>sm eq. inv sm.
   econstructor...
   apply: conv_trans...
 Qed.
 
-Lemma sim_transR x y z : sim x y -> z === x -> sim z y.
+Lemma sim_transR x y z : sim x y -> z ≃ x -> sim z y.
 Proof with eauto using head_sim.
   move=>sm eq. inv sm.
   econstructor.
@@ -126,7 +127,7 @@ Ltac solve_sim :=
   end;
   try solve[solve_conv];
   match goal with
-  | [ eq1 : ?x === ?z, eq2 : ?z === ?y |- _ ] =>
+  | [ eq1 : ?x ≃ ?z, eq2 : ?z ≃ ?y |- _ ] =>
     pose proof (conv_trans _ eq1 eq2); solve_conv
   end.
 
@@ -149,6 +150,8 @@ Proof with eauto.
   { move=>A m n1 n2 s t eq1 eq2.
     have/sort_inj//:=conv_trans _ eq1 eq2. }
   { move=>m n s t eq1 eq2.
+    have/sort_inj//:=conv_trans _ eq1 eq2. }
+  { move=>m n eq1 eq2. 
     have/sort_inj//:=conv_trans _ eq1 eq2. }
 Qed.
 
@@ -178,6 +181,9 @@ Proof with eauto using sim.
     have/pi0_inj[eqA[eqB->]]:=conv_trans _ eq1 eq2.
     repeat split... }
   { move=>m n A1 A2 B1 B2 s1 s2 eq1 eq2.
+    have/pi0_inj[eqA[eqB->]]:=conv_trans _ eq1 eq2.
+    repeat split... }
+  { move=>A1 A2 B1 B2 s1 s2 eq1 eq2.
     have/pi0_inj[eqA[eqB->]]:=conv_trans _ eq1 eq2.
     repeat split... }
 Qed.
@@ -210,11 +216,14 @@ Proof with eauto using sim.
   { move=>m n A1 A2 B1 B2 s1 s2 eq1 eq2.
     have/pi1_inj[eqA[eqB->]]:=conv_trans _ eq1 eq2.
     repeat split... }
+  { move=>A1 A2 B1 B2 s1 s2 eq1 eq2.
+    have/pi1_inj[eqA[eqB->]]:=conv_trans _ eq1 eq2.
+    repeat split... }
 Qed.
 
 Lemma sim_act0_inj A1 A2 B1 B2 r1 r2 :
   sim (Act0 r1 A1 B1) (Act0 r2 A2 B2) ->
-    A1 === A2 /\ B1 === B2 /\  r1 = r2.
+    A1 ≃ A2 /\ B1 ≃ B2 /\  r1 = r2.
 Proof with eauto.
   move=>sm. inv sm.
   elim: H0 A1 A2 B1 B2 r1 r2 H H1=>{x y}.
@@ -232,6 +241,8 @@ Proof with eauto.
   { move=>m n A1 A2 B1 B2 r1 r2 eq1 eq2.
     have/act0_inj//:=conv_trans _ eq1 eq2. }
   { move=>r A B A1 A2 B1 B2 r1 r2 eq1 eq2.
+    have/act0_inj//:=conv_trans _ eq1 eq2. }
+  { move=>A1 A2 B1 B2 r1 r2 eq1 eq2.
     have/act0_inj//:=conv_trans _ eq1 eq2. }
 Qed.
 
